Complete admitted proofs for soundness of interpreter.

src/interpreter.v
@@ -31,15 +31,53 @@ Proof.
     * intros t Hterm. simpl. simpl in Hterm. destruct (observe t) eqn:Heq; eauto.
 Qed.
 
-Lemma exec_eutt {R} n (t t' : itree voidE R) r :
-  t ≈ t' →
-  exec n t = Some r →
-  ∃ n', exec n' t' = Some r.
+Lemma exec_agree {R} n m r1 r2 (t : itree voidE R) :
+  exec m t = Some r1 →
+  exec n t = Some r2 →
+  r1 = r2.
 Proof.
-  intros Heutt Hexec.
-  destruct n as [|n]. { discriminate. }
-  induction n.
-Admitted.
+  intros Hr1 Hr2.
+  destruct (decide (n ≤ m)) as [Hlt|Hgt].
+  - rewrite (exec_stable m n) // Hr2 in Hr1. by injection Hr1.
+  - rewrite (exec_stable n m) // in Hr2; last lia. rewrite Hr1 in Hr2. by injection Hr2.
+Qed.
+
+Inductive returns' {R} : itree' voidE R → R → Prop :=
+  | returns_Tau t r :
+  returns' (observe t) r →
+  returns' (TauF t) r
+  | returns_Ret r :
+  returns' (RetF r) r.
+Definition returns {R} (t : itree voidE R) (r : R) : Prop :=
+  returns' (observe t) r.
+
+Lemma eutt_returns {R} t (r : R) :
+  t ≈ Ret r →
+  returns t r.
+Proof.
+  intros Heutt. rewrite /eutt in Heutt. rewrite /eqit in Heutt. punfold Heutt.
+  rewrite /returns.
+  rewrite /eqit_ in Heutt. simpl in Heutt. remember (RetF r) as t'.
+  induction Heutt; simplify_eq.
+  - constructor.
+  - constructor. by apply IHHeutt.
+Qed.
+
+Lemma exec_ret {R} (t : itree voidE R) r :
+  t ≈ Ret r →
+  ∃ n, exec n t = Some r.
+Proof.
+  intros Hret%eutt_returns.
+  rewrite /returns in Hret.
+  remember (observe t) as ot.
+  revert t Heqot.
+  induction Hret.
+  - intros t' Heqot. destruct (observe t') eqn:Heq; try discriminate. simplify_eq.
+    odestruct (IHHret t0 _) as [n Hexec]; first done. exists (S n).
+    rewrite /= Heq //.
+  - intros t' Heqot. destruct (observe t') eqn:Heq; try discriminate. simplify_eq.
+    exists 1. rewrite /= Heq //.
+Qed.
 
 Lemma exec_soundness' `{!invGS_gen hlc Σ} {R} M (t : itree voidE R) Φ :
   WPi t @ voidH; M {{ v, ⌜Φ v⌝ }} -∗
@@ -48,8 +86,8 @@ Proof.
   iIntros "Hwp".
   iMod (voidE_terminates with "Hwp") as "[%v [%Heutt HΦ]]".
   iModIntro. iMod "HΦ". iModIntro. iDestruct "HΦ" as "%HΦ".
-  iPureIntro. symmetry in Heutt.
-  apply exec_eutt with (n := 1) (r := v) in Heutt as [n Hexec]; last done.
+  iPureIntro.
+  apply exec_ret in Heutt as [n Hexec].
   by exists n, v.
 Qed.
 
